Msg refactor, LimitedCounter

random/Elmo.hs
@@ -1,0 +1,19 @@
+type Model = Int
+
+init :: Model
+init = 0
+
+type Msg = Increment | Decrement
+
+update :: Model -> Msg -> Model
+update model = \case
+  Increment -> model + 1
+  Decrement -> model - 1
+
+view : Model -> Html Msg
+view model =
+  div []
+    [ button [ onClick Decrement ] [ text "-" ]
+    , div [] [ text (show model) ]
+    , button [ onClick Increment ] [ text "+" ]
+    ]
