random/Examples.hs
@@ -1,0 +1,18 @@
+
+type Key = Natural
+
+data Map v
+  = Branch Key v (Map v) (Map v)
+  | Leaf
+
+isEmpty :: Map v -> Bool
+isEmpty m =
+  case m of
+    Branch _ _ _ _ -> False
+    Leaf -> True
+
+size :: Map v -> Natural
+size m =
+  case m of
+    Branch _ _ l r -> 1 + size l + size r
+    Leaf -> 0
