src/limited_counter_main.ml
@@ -1,0 +1,15 @@
+open Tea.App
+open LimitedCounter
+
+let _ = 
+  Js.Global.setTimeout
+    (fun _ -> 
+
+    beginnerProgram {
+      model = App.init ();
+      update = App.update;
+      view = App.view;
+    } (Web.Document.getElementById "app") () 
+    |. ignore
+    )  
+  0
