src/Counter.v
@@ -17,13 +17,13 @@ Module Model.
   Definition t := Model.
 End Model.
 
-Inductive event :=
-  | Increment : event
-  | Decrement : event.
+Inductive Msg :=
+  | Increment : Msg
+  | Decrement : Msg.
 
 Definition init (_ : unit) : Model.t := 0.
 
-Definition update (m : Model.t) (msg : event) : Model.t :=
+Definition update (m : Model.t) (msg : Msg) : Model.t :=
   match msg with
   | Increment => m + 1
   | Decrement => m - 1
@@ -31,7 +31,7 @@ Definition update (m : Model.t) (msg : event) : Model.t :=
 
 Definition string_of_nat (n : nat) : string := NilZero.string_of_uint (Nat.to_uint n).
 
-Definition view (m : Model.t) : html event :=
+Definition view (m : Model.t) : html Msg :=
   el "div"
     []
     [ el "button"
@@ -40,12 +40,9 @@ Definition view (m : Model.t) : html event :=
     ; el "span"
          [ "class"=:"count" ]
          [ text (string_of_nat m) ]
-    ; if m <? 10 then
-        el "button"
-          [ on "click" Increment ]
-          [ text "+" ]
-      else
-        text "can't increment"
+    ; el "button"
+        [ on "click" Increment ]
+        [ text "+" ]
     ].
 
 End App.
@@ -54,31 +51,19 @@ Module Proofs.
 
 Import App.
 
-Theorem can_always_increment : forall m, m < 10 -> Html.event_possible Increment (view m).
-  intros m Hm.
-  unfold view.
-  try rewrite (proj2 (Nat.ltb_lt m 10) Hm).
-  find_event auto.
+Theorem can_always_increment : forall m, Html.msg_possible Increment (view m).
+  intros.
+  find_msg auto.
 Qed.
 
 Theorem can_go_to_5 : reachable (fun m => m = 5) (init tt) update view.
 Proof.
-  do 5 (apply (R_Step update view Increment); simpl; try (find_event auto)).
+  do 5 (apply (R_Step update view Increment); simpl; try (find_msg auto)).
   apply R_Here.
   reflexivity.
 Qed.
 
-Theorem cant_go_to_15 : ~ reachable (fun m => m = 15) (init tt) update view.
-Proof.
-  apply (not_reachable_if_invariant_violated (fun m => m < 10)).
-
-  constructor.
-
-  unfold init. apply Nat.lt_0_succ.
-
-Admitted.
-
-Lemma can_go_to_any_number : forall n, Html.reachable (fun m => m = n) (init tt) update view.
+Theorem can_go_to_any_number : forall n, Html.reachable (fun m => m = n) (init tt) update view.
 Proof.
   assert (can_go_from_k : forall n k, Html.reachable (fun m => m = n + k) k update view).
   intros n.
@@ -86,7 +71,7 @@ Proof.
 
   apply R_Here. reflexivity.
 
-  apply (R_Step update view Increment); try (find_event auto). simpl.
+  apply (R_Step update view Increment); try (find_msg auto). simpl.
   rewrite <- PeanoNat.Nat.add_succ_r.
   rewrite PeanoNat.Nat.add_1_r.
   apply (IHn (S k)).
