src/Html.v
@@ -81,27 +81,26 @@ Fixpoint any {A : Type} (p: A -> Prop) (xs: list A) : Prop :=
   | x :: xs => p x \/ any p xs
   end.
 
-Definition event_possible_from_prop {A : Set} (x : A) (p: hprop A) : Prop :=
+Definition msg_possible_from_prop {A : Set} (x : A) (p: hprop A) : Prop :=
   match p with
   | Event _ _ _ decoder =>
       Decoder.value_possible x decoder
   | _ => False
   end.
 
-Inductive event_possible {A: Set} (x : A) : html A -> Prop :=
+Inductive msg_possible {A: Set} (x : A) : html A -> Prop :=
   | EP_Prop : forall tag props children,
-      any (event_possible_from_prop x) props -> event_possible x (Elem A tag props children)
+      any (msg_possible_from_prop x) props -> msg_possible x (Elem A tag props children)
   | EP_Children : forall tag props children,
-      event_possible_list x children -> event_possible x (Elem A tag props children)
-with event_possible_list {A: Set} (x : A) : list (html A) -> Prop :=
-  | EP_Here : forall h rest, event_possible x h -> event_possible_list x (h :: rest)
-  | EP_Next : forall h rest, event_possible_list x rest -> event_possible_list x (h :: rest).
-
+      msg_possible_list x children -> msg_possible x (Elem A tag props children)
+with msg_possible_list {A: Set} (x : A) : list (html A) -> Prop :=
+  | EP_Here : forall h rest, msg_possible x h -> msg_possible_list x (h :: rest)
+  | EP_Next : forall h rest, msg_possible_list x rest -> msg_possible_list x (h :: rest).
 
 Inductive reachable {M E : Set} (P : M -> Prop) (from : M) (update : M -> E -> M) (view : M -> html E) : Prop :=
   | R_Here : P from -> reachable P from update view
   | R_Step : forall event,
-      event_possible event (view from) ->
+      msg_possible event (view from) ->
       reachable P (update from event) update view ->
       reachable P from update view.
 
@@ -109,38 +108,28 @@ Arguments R_Step {_ _ _ _}.
 
 Hint Unfold any el on on_with_opts Decoder.heq : core.
 
-Ltac find_event t :=
+Ltac find_msg t :=
   simpl; solve
     [ apply EP_Prop; simpl; t
-    | apply EP_Here; t; find_event t
-    | apply EP_Next; t; find_event t
-    | apply EP_Children; t; find_event t ].
+    | apply EP_Here; t; find_msg t
+    | apply EP_Next; t; find_msg t
+    | apply EP_Children; t; find_msg t ].
 
 
-Inductive always {M E : Set} (P : M -> Prop) (from : M) (update : M -> E -> M) (view : M -> html E) : Prop :=
-  | Always :
-     P from ->
-     (forall event,
-         event_possible event (view from) ->
-         always P (update from event) update view) ->
-     always P from update view.
+Definition always {M E : Set} (P : M -> Prop) (from : M) (update : M -> E -> M) (view : M -> html E) : Prop :=
+  P from /\ (forall m msg, P m -> msg_possible msg (view m) -> P (update m msg)).
 
 Theorem not_reachable_if_invariant_violated {M E : Set} (P : M -> Prop) (from : M) (update : M -> E -> M) (view : M -> html E) (P2 : M -> Prop) :
   always P from update view -> (forall m, P2 m -> ~ P m) -> ~ reachable P2 from update view.
 Proof.
   intros Halways Hno_invariant.
+  destruct Halways as [Hinitial Hstep].
   intro H.
   induction H.
 
-  destruct Halways.
   apply (Hno_invariant from H).
-  auto.
+  assumption.
 
-  apply IHreachable.
-  destruct Halways.
-  apply Always.
-  apply (H2 event); auto.
-
-  intros.
-  apply (H2 event); auto.
+  apply IHreachable; try assumption.
+  apply (Hstep from event Hinitial H).
  Qed.
