random/Examples.v
@@ -1,0 +1,21 @@
+
+Definition key := nat.
+
+Inductive map (V : Set) :=
+  | Branch : key -> V -> map V -> map V -> map V
+  | Leaf : map V.
+
+Arguments Branch {_}.
+Arguments Leaf {_}.
+
+Definition is_empty {V} (m : map V) : bool :=
+  match m with
+  | Branch _ _ _ _ => false
+  | Leaf => true
+  end.
+
+Fixpoint size {V} (m : map V) : nat :=
+  match m with
+  | Branch _ _ l r => 1 + size l + size r
+  | Leaf => 0
+  end.
