src/LimitedCounter.v
@@ -1,0 +1,126 @@
+Require Import String.
+Require Import DecimalString.
+Require Import List.
+Require Import PeanoNat.
+
+Import ListNotations.
+Open Scope string_scope.
+Open Scope list_scope.
+
+Require Import Html.
+
+Module App.
+
+Definition Model := nat.
+
+Module Model.
+  Definition t := Model.
+End Model.
+
+Inductive Msg :=
+  | Increment : Msg
+  | Decrement : Msg.
+
+Definition init (_ : unit) : Model.t := 0.
+
+Definition update (m : Model.t) (msg : Msg) : Model.t :=
+  match msg with
+  | Increment => m + 1
+  | Decrement => m - 1
+  end.
+
+Definition string_of_nat (n : nat) : string := NilZero.string_of_uint (Nat.to_uint n).
+
+Definition view (m : Model.t) : html Msg :=
+  el "div"
+    []
+    [ el "button"
+         [ on "click" Decrement ]
+         [ text "-" ]
+    ; el "span"
+         [ "class"=:"count" ]
+         [ text (string_of_nat m) ]
+    ; if m <? 10 then
+        el "button"
+          [ on "click" Increment ]
+          [ text "+" ]
+      else
+        text "can't increment"
+    ].
+
+End App.
+
+Module Proofs.
+
+Import App.
+
+Theorem can_increment_if_below_limit : forall m, m < 10 -> Html.msg_possible Increment (view m).
+  intros m Hm.
+  unfold view.
+  try rewrite (proj2 (Nat.ltb_lt m 10) Hm).
+  find_msg auto.
+Qed.
+
+Lemma not_any_empty : forall {A} (P : A -> Prop), any P [] -> False.
+Proof.
+  auto.
+Qed.
+
+Ltac msg_impossible :=
+  match goal with
+  | H : any ?P [] |- False => apply (not_any_empty P); assumption
+  | H : any (msg_possible_from_prop _) _ |- False => inversion H; clear H
+  | H : msg_possible _ _ |- False => inversion H; clear H
+  | H : msg_possible_list _ _ |- False => inversion H; clear H
+  | H : msg_possible_from_prop _ _ |- False => inversion H; clear H
+  end.
+
+Theorem cant_increment_if_at_limit : ~ Html.msg_possible Increment (view 10).
+  intros Hpossible.
+  repeat msg_impossible.
+Qed.
+
+Theorem can_go_to_5 : reachable (fun m => m = 5) (init tt) update view.
+Proof.
+  do 5 (apply (R_Step update view Increment); simpl; try (find_msg auto)).
+  apply R_Here.
+  reflexivity.
+Qed.
+
+
+Theorem always_le_10 : always (fun m => m <= 10) (init tt) update view.
+Proof.
+  constructor.
+  apply Nat.le_0_l.
+
+  intros m msg Hlt10 Hpossible.
+  destruct msg.
+  destruct (Nat.eq_decidable m 10).
+  exfalso.
+  rewrite H in *.
+  apply (cant_increment_if_at_limit Hpossible).
+  inversion Hlt10.
+  exfalso. auto.
+  unfold update.
+  rewrite Nat.add_1_r.
+  Search le S.
+  apply le_n_S.
+  assumption.
+
+  simpl.
+  rewrite Nat.le_sub_le_add_r.
+  simpl.
+  auto.
+Qed.
+
+Theorem cant_go_to_15 : ~ reachable (fun m => m = 15) (init tt) update view.
+Proof.
+  apply (not_reachable_if_invariant_violated (fun m => m <= 10)).
+  apply always_le_10.
+
+  intros m Hm15. rewrite Hm15 in *.
+  apply (proj1 (Nat.leb_nle 15 10)).
+  reflexivity.
+Qed.
+
+End Proofs.
